AwsCryptographicMaterialProviders/dafny/AwsCryptographyKeyStoreAdmin/src/KeyStoreAdminErrorMessages.dfy
@@ -3,7 +3,7 @@
 
 module {:options "/functionSyntax:4" } KeyStoreAdminErrorMessages {
   const NO_MUTATE_TO_HV_1: string :=
-    "At this time, a Mutation cannot change a Branch Key from HV-2 to HV-1. The request dictated 'TerminalHierarchyVersion := v1' and was therefore rejected. Remove the 'TerminalHierarchyVersion' parameter or set it to at least 'v2'."
+    "At this time, a Mutation cannot downgrade a Branch Key from HV-2 to HV-1. The request attempted to downgrade from HV-2 by setting 'TerminalHierarchyVersion := v1', which is not allowed."
 
   const UNSUPPORTED_KEY_MANAGEMENT_STRATEGY :=
     "Unsupported KeyManagementStrategy."
